Create test, but not working

rupicola/io/RunningExample.fst
@@ -21,5 +21,22 @@ let wrapper f task agent =
   then io_return (Inl ())
   else io_return (Inr ())
 
+val good_agent_aux : string -> string -> io (resexn unit)
+let good_agent_aux fn task =
+  let!@! fd = openfile fn in
+  let!@! data = read fd in
+  write (fd, data ^ task)
+
+val good_agent : string -> string -> io unit
+let good_agent fn task =
+  let!@ r = good_agent_aux fn task in
+  io_return ()
+
+let test () =
+  wrapper "bla" "st" good_agent
+
+[@expect_failure]
+%splice_t[tgt_test] (meta_translation "tgt_test" [`test])
+
 [@expect_failure]
 %splice_t[tgt_wrapper] (meta_translation "tgt_wrapper" [`wrapper])
